src/Undefined.v
@@ -87,6 +87,6 @@ Definition undefined_list {T} `{Inhabited T} (a:T) : monad rv (list T) E :=
   undefined_nat tt >>= fun n =>
   returnm (repeat (List.cons a List.nil) n).
   
-Definition undefined_vector {T} n `{Inhabited T} (a:T) : monad rv (vec T n) E := returnm (vec_init a n).
+Definition undefined_vector {T} n `{Inhabited T} (a:T) : monad rv (vec T n) E := returnm (vector_init n a).
 
 End Undef.
